Port Lock's RefinementProof.i.dfy to concur-tree style

ironfleet/src/Dafny/Distributed/Protocol/Lock/RefinementProof/RefinementProof.i.dfy
@@ -9,15 +9,15 @@ module RefinementProof_i {
     import opened Collections__Maps_i
     import opened Logic__Option_i
 
-    lemma lemma_InitRefines(gls:GLS_State, config:Config) 
-        requires GLS_Init(gls, config);
-        ensures  Service_Init(AbstractifyGLS_State(gls), UniqueSeqToSet(config));
+    lemma lemma_InitRefines(gls:GLockSystemState, config:LockConfig) 
+        requires GLockSystemInit(config, gls);
+        ensures  Service_Init(AbstractifyGLockSystemState(gls), UniqueSeqToSet(config));
     {
         assert config[0] in config; // OBSERVE: triggers the exists in Service_Init
-        var s := AbstractifyGLS_State(gls);
+        var s := AbstractifyGLockSystemState(gls);
         calc {
             s.hosts;
-            mapdomain(gls.ls.servers);
+            mapdomain(gls.ls.states);
             UniqueSeqToSet(config);
         }
 
@@ -25,116 +25,116 @@ module RefinementProof_i {
         assert config[0] in UniqueSeqToSet(config);
     }
 
-    predicate IsValidBehavior(glb:seq<GLS_State>, config:Config)
+    predicate IsValidBehavior(glb:seq<GLockSystemState>, config:LockConfig)
     {
         |glb| > 0
-     && GLS_Init(glb[0], config)
-     && (forall i {:trigger GLS_Next(glb[i], glb[i+1])} :: 0 <= i < |glb| - 1 ==> GLS_Next(glb[i], glb[i+1]))
+     && GLockSystemInit(config, glb[0])
+     && (forall i {:trigger GLockSystemNext(glb[i], glb[i+1])} :: 0 <= i < |glb| - 1 ==> GLockSystemNext(glb[i], glb[i+1]))
     }
 
-    lemma lemma_LS_Next(glb:seq<GLS_State>, config:Config, i:int)
+    lemma lemma_LockSystemNext(glb:seq<GLockSystemState>, config:LockConfig, i:int)
         requires IsValidBehavior(glb, config);
         requires 0 <= i < |glb| - 1;
-        ensures  GLS_Next(glb[i], glb[i+1]);
+        ensures  GLockSystemNext(glb[i], glb[i+1]);
     {
     }
 
-    lemma lemma_LSConsistent(glb:seq<GLS_State>, config:Config, i:int)
+    lemma lemma_LSConsistent(glb:seq<GLockSystemState>, config:LockConfig, i:int)
         requires IsValidBehavior(glb, config);
         requires 0 <= i < |glb|;
-        ensures  |glb[i].ls.servers| == |config|;
-        ensures  forall e :: e in config <==> e in glb[i].ls.servers;
-        ensures  mapdomain(glb[i].ls.servers) == mapdomain(glb[0].ls.servers);
-        ensures  forall id :: id in config ==> glb[0].ls.servers[id].config == glb[i].ls.servers[id].config;
+        ensures  |glb[i].ls.states| == |config|;
+        ensures  forall e :: e in config <==> e in glb[i].ls.states;
+        ensures  mapdomain(glb[i].ls.states) == mapdomain(glb[0].ls.states);
+        ensures  forall id :: id in config ==> glb[0].ls.states[id].config == glb[i].ls.states[id].config;
     {
         if i == 0 {
             calc {
                 UniqueSeqToSet(config);
-                mapdomain(glb[0].ls.servers);
+                mapdomain(glb[0].ls.states);
             }
-            lemma_seqs_set_cardinality(config, mapdomain(glb[0].ls.servers));
+            lemma_seqs_set_cardinality(config, mapdomain(glb[0].ls.states));
             calc {
-                |mapdomain(glb[0].ls.servers)|;
-                    { lemma_MapSizeIsDomainSize(mapdomain(glb[0].ls.servers), glb[0].ls.servers); }
-                |glb[0].ls.servers|;
+                |mapdomain(glb[0].ls.states)|;
+                    { lemma_MapSizeIsDomainSize(mapdomain(glb[0].ls.states), glb[0].ls.states); }
+                |glb[0].ls.states|;
             }
         } else {
-            lemma_LS_Next(glb, config, i - 1);
+            lemma_LockSystemNext(glb, config, i - 1);
             lemma_LSConsistent(glb, config, i - 1);
         }
     }
 
-    lemma lemma_LSNodeConsistent(glb:seq<GLS_State>, config:Config, i:int, candidate:EndPoint, e:EndPoint)
+    lemma lemma_LSNodeConsistent(glb:seq<GLockSystemState>, config:LockConfig, i:int, candidate:EndPoint, e:EndPoint)
         requires IsValidBehavior(glb, config);
         requires 0 <= i < |glb|;
-        requires e in glb[i].ls.servers;
-        ensures  candidate in glb[i].ls.servers <==> candidate in glb[i].ls.servers[e].config;
+        requires e in glb[i].ls.states;
+        ensures  candidate in glb[i].ls.states <==> candidate in glb[i].ls.states[e].config;
     {
         if i == 0 {
         } else {
-            lemma_LS_Next(glb, config, i-1);
+            lemma_LockSystemNext(glb, config, i-1);
             lemma_LSConsistent(glb, config, i-1);
             lemma_LSNodeConsistent(glb, config, i-1, candidate, e);
         }
     }
 
-    lemma lemma_HistoryIncrement(glb:seq<GLS_State>, config:Config, i:int)
+    lemma lemma_HistoryIncrement(glb:seq<GLockSystemState>, config:LockConfig, i:int)
         requires IsValidBehavior(glb, config);
         requires 0 <= i < |glb| - 1;
         ensures  |glb[i].history| + 1 == |glb[i].history|
               || glb[i].history == glb[i].history;
     { }
 
-    lemma lemma_HistorySize(glb:seq<GLS_State>, config:Config, i:int)
+    lemma lemma_HistorySize(glb:seq<GLockSystemState>, config:LockConfig, i:int)
         requires IsValidBehavior(glb, config);
         requires 0 <= i < |glb|;
         ensures  1 <= |glb[i].history| <= i + 1;
     { 
         if i == 0 {
-            var locked_packets := set p | p in glb[i].ls.environment.sentPackets && p.msg.Locked?;
+            var locked_packets := set p | p in glb[i].ls.sent_packets && p.msg.Locked?;
             assert |locked_packets| == 0;
-            assert exists host :: host in (glb[i]).ls.servers && (glb[i]).ls.servers[host].held;
+            assert exists host :: host in (glb[i]).ls.states && (glb[i]).ls.states[host].held;
             assert |glb[i].history| == 1;
         } else {
             lemma_HistorySize(glb, config, i - 1);
             lemma_HistoryIncrement(glb, config, i - 1);
-            assert GLS_Next(glb[i-1], glb[i]);
+            assert GLockSystemNext(glb[i-1], glb[i]);
         }
     }
 
-    lemma lemma_HistoryMembership(glb:seq<GLS_State>, config:Config, i:int)
+    lemma lemma_HistoryMembership(glb:seq<GLockSystemState>, config:LockConfig, i:int)
         requires IsValidBehavior(glb, config);
         requires 0 <= i < |glb|;
         ensures  1 <= |glb[i].history| <= i + 1;
-        ensures  last(glb[i].history) in glb[i].ls.servers;
+        ensures  last(glb[i].history) in glb[i].ls.states;
     {
         lemma_HistorySize(glb, config, i);
 
         if i == 0 { 
         } else {
-            lemma_LS_Next(glb, config, i - 1);
+            lemma_LockSystemNext(glb, config, i - 1);
             lemma_LSConsistent(glb, config, i - 1);
             lemma_LSConsistent(glb, config, i);
             lemma_HistoryMembership(glb, config, i-1);
         }
     }
 
-    lemma lemma_LS_NextAbstract(glb:seq<GLS_State>, config:Config, i:int)
+    lemma lemma_LockSystemNextAbstract(glb:seq<GLockSystemState>, config:LockConfig, i:int)
         requires IsValidBehavior(glb, config);
         requires 0 <= i < |glb| - 1;
-        ensures  Service_Next(AbstractifyGLS_State(glb[i]), AbstractifyGLS_State(glb[i+1]))
-               || AbstractifyGLS_State(glb[i]) == AbstractifyGLS_State(glb[i+1]);
+        ensures  Service_Next(AbstractifyGLockSystemState(glb[i]), AbstractifyGLockSystemState(glb[i+1]))
+               || AbstractifyGLockSystemState(glb[i]) == AbstractifyGLockSystemState(glb[i+1]);
     {
         lemma_LSConsistent(glb, config, i);
         lemma_LSConsistent(glb, config, i+1);
-        assert GLS_Next(glb[i], glb[i+1]);
+        assert GLockSystemNext(glb[i], glb[i+1]);
         if i == 0 {
-            assert glb[i].ls.servers[config[0]].held;
+            assert glb[i].ls.states[config[0]].held;
         } else {
             lemma_HistorySize(glb, config, i);
             assert |glb[i].history| > 0;
             lemma_HistoryMembership(glb, config, i);
-            assert last(glb[i].history) in glb[i].ls.servers;
+            assert last(glb[i].history) in glb[i].ls.states;
         }
     }
 
@@ -144,36 +144,37 @@ module RefinementProof_i {
     ///  needed to prove Service_Correspondence.
     ///////////////////////////////////////////////////////////////////
 
-    lemma MakeLockHistory(glb:seq<GLS_State>, config:Config, i:int) returns (history:seq<EndPoint>)
+    lemma MakeLockHistory(glb:seq<GLockSystemState>, config:LockConfig, i:int) returns (history:seq<EndPoint>)
         requires IsValidBehavior(glb, config);
         requires 0 <= i < |glb|;
         ensures |history| > 0;
-        ensures forall p :: p in glb[i].ls.environment.sentPackets && p.msg.Transfer? && p.src in glb[i].ls.servers 
+        ensures forall p :: p in glb[i].ls.sent_packets && p.msg.Transfer? && p.src in glb[i].ls.states 
                         ==> 2 <= p.msg.transfer_epoch <= |history|;
-        ensures forall p :: p in glb[i].ls.environment.sentPackets && p.msg.Transfer? && p.src in glb[i].ls.servers 
+        ensures forall p :: p in glb[i].ls.sent_packets && p.msg.Transfer? && p.src in glb[i].ls.states 
                         ==> history[p.msg.transfer_epoch-1] == p.dst;
-        ensures forall h,j :: h in glb[i].ls.servers && 0 <= j < |history|-1 && history[j] == h ==> j+1 <= glb[i].ls.servers[h].epoch;
-        ensures forall h :: h in glb[i].ls.servers && h != last(history) ==> !glb[i].ls.servers[h].held;
-        ensures forall h :: h in glb[i].ls.servers && glb[i].ls.servers[h].held ==> glb[i].ls.servers[h].epoch == |history|;
+        ensures forall h,j :: h in glb[i].ls.states && 0 <= j < |history|-1 && history[j] == h ==> j+1 <= glb[i].ls.states[h].epoch;
+        ensures forall h :: h in glb[i].ls.states && h != last(history) ==> !glb[i].ls.states[h].held;
+        ensures forall h :: h in glb[i].ls.states && glb[i].ls.states[h].held ==> glb[i].ls.states[h].epoch == |history|;
         ensures history == glb[i].history;
     {
         if i == 0 {
             history := [config[0]];
         } else {
             var prevHistory := MakeLockHistory(glb, config, i-1);
-            lemma_LS_Next(glb, config, i-1);
+            lemma_LockSystemNext(glb, config, i-1);
             lemma_LSConsistent(glb, config, i-1);
             lemma_LSConsistent(glb, config, i);
             var s := glb[i-1];
             var s' := glb[i];
-            assert LEnvironment_Next(s.ls.environment, s'.ls.environment);
+
+            var entry :| GLockSystemNextEntry(s, s', entry);
             
-            if s.ls.environment.nextStep.LEnvStepHostIos? && s.ls.environment.nextStep.actor in s.ls.servers {
-                var id := s.ls.environment.nextStep.actor;
-                var ios := s.ls.environment.nextStep.ios;
+            if entry.action.LockActionHostNext? && entry.actor.ep in s.ls.states {
+                var id := entry.actor.ep;
+                var ios := entry.action.ios;
                 
-                if NodeGrant(s.ls.servers[id], s'.ls.servers[id], ios) {
-                    if s.ls.servers[id].held && s.ls.servers[id].epoch < 0xFFFF_FFFF_FFFF_FFFF {
+                if NodeGrant(s.ls.states[id], s'.ls.states[id], ios) {
+                    if s.ls.states[id].held && s.ls.states[id].epoch < 0xFFFF_FFFF_FFFF_FFFF {
                         history := prevHistory + [ios[0].s.dst];
                     } else {
                         history := prevHistory;
@@ -181,13 +182,12 @@ module RefinementProof_i {
                 } else {
                     history := prevHistory;
                     
-                    if   !ios[0].LIoOpTimeoutReceive? 
-                      && !s.ls.servers[id].held 
-                      && ios[0].r.src in s.ls.servers[id].config
+                    if   !ios[0].LockIoTimeoutReceive?
+                      && !s.ls.states[id].held 
+                      && ios[0].r.src in s.ls.states[id].config
                       && ios[0].r.msg.Transfer? 
-                      && ios[0].r.msg.transfer_epoch > s.ls.servers[id].epoch {
+                      && ios[0].r.msg.transfer_epoch > s.ls.states[id].epoch {
                         var p := ios[0].r;
-                        assert IsValidLIoOp(ios[0], id, s.ls.environment);     // trigger
                         assert p.dst == id;
                     }
                 }
@@ -196,4 +196,5 @@ module RefinementProof_i {
             }
         }
     }
+
 }
